Cleaned up unused utils

00Utils/Utils.thy
@@ -4,21 +4,22 @@ begin
 
 section \<open>Utilities\<close>
 
-text \<open>
-In this section we have a number of miscellaneous functions and lemmas about the standard library 
-that do not fit anywhere else.
-\<close>
+text \<open>We begin with a small collection of utility functions. Most of this can be skimmed on a first 
+read.\<close>
+
+subsection \<open>Utilities\<close>
+
+text \<open>In this section we have a number of miscellaneous functions and lemmas about the standard 
+library that do not fit anywhere else.\<close>
 
 lemma dom_expanded_fun_upd [simp]: "dom (\<lambda>a. if a = x then Some y else f a) = insert x (dom f)"
   by (auto simp add: dom_if)
 
-lemma [simp]: "ran (map_option f \<circ> g) = f ` ran g"
+lemma ran_of_map_option [simp]: "ran (map_option f \<circ> g) = f ` ran g"
   by (auto simp add: ran_def)
 
-lemma [simp]: "map_option Suc opt \<noteq> Some 0"
-  by (induction opt) simp_all
-
-lemma [simp]: "image_mset fst (mset ab) = add_mset a s \<Longrightarrow> Some (the (map_of ab a)) = map_of ab a"
+lemma some_the_map_of_cancel [simp]: "image_mset fst (mset ab) = add_mset a s \<Longrightarrow> 
+  Some (the (map_of ab a)) = map_of ab a"
 proof (induction ab arbitrary: s)
   case (Cons ab abb)
   thus ?case
@@ -35,10 +36,10 @@ proof (induction ab arbitrary: s)
   qed
 qed simp_all
 
-lemma [simp]: "length (concat (map f as)) = sum_list (map (length \<circ> f) as)"
+lemma length_concat_map [simp]: "length (concat (map f as)) = sum_list (map (length \<circ> f) as)"
   by (induction as) simp_all
 
-lemma [simp]: "length as \<noteq> length bs \<Longrightarrow> map f as \<noteq> map f bs"
+lemma length_neq_map_neq [simp]: "length as \<noteq> length bs \<Longrightarrow> map f as \<noteq> map f bs"
 proof (induction as arbitrary: bs)
   case Nil
   thus ?case by (induction bs) simp_all
@@ -47,26 +48,22 @@ next
   thus ?case by (induction bs) simp_all
 qed
 
-lemma [simp]: "finite as \<Longrightarrow> x \<in> as \<Longrightarrow> 0 < card as"
-  by (induction "card as") simp_all
-
-lemma [simp]: "finite as \<Longrightarrow> a \<in> as \<Longrightarrow> Suc (card as - Suc 0) = card as"
-  by (induction as rule: finite_induct) simp_all
-
-lemma [simp]: "finite as \<Longrightarrow> finite bs \<Longrightarrow> card as < Suc (card (bs \<union> as))"
+lemma finite_card_union' [simp]: "finite as \<Longrightarrow> finite bs \<Longrightarrow> card as < Suc (card (bs \<union> as))"
 proof -
   assume "finite as" and "finite bs"
   hence "card as \<le> card (bs \<union> as)" by (simp add: card_mono)
   thus ?thesis by simp
 qed
 
-lemma [simp]: "finite as \<Longrightarrow> finite bs \<Longrightarrow> x \<in> as \<Longrightarrow> x \<notin> bs \<Longrightarrow> card bs < card (as \<union> bs)"
+lemma finite_card_union [simp]: "finite as \<Longrightarrow> finite bs \<Longrightarrow> x \<in> as \<Longrightarrow> x \<notin> bs \<Longrightarrow> 
+  card bs < card (as \<union> bs)"
 proof (induction as arbitrary: bs rule: finite_induct)
   case (insert a as)
   thus ?case by (cases "x = a") (simp_all add: card_insert_if)
 qed simp_all
 
-lemma [simp]: "finite as \<Longrightarrow> finite bs \<Longrightarrow> x \<notin> as \<Longrightarrow> x \<in> bs \<Longrightarrow> card (bs - {x} \<union> as) < card (as \<union> bs)"
+lemma finite_card_union_remove [simp]: "finite as \<Longrightarrow> finite bs \<Longrightarrow> x \<notin> as \<Longrightarrow> x \<in> bs \<Longrightarrow> 
+  card (bs - {x} \<union> as) < card (as \<union> bs)"
 proof -
   assume "finite as" and "finite bs" and "x \<in> bs"
   moreover hence "card (insert x (as \<union> bs)) = card (as \<union> bs)" by (simp add: card_insert_if)
@@ -74,49 +71,26 @@ proof -
   ultimately show ?thesis by (simp add: Un_Diff card.insert_remove sup_commute)
 qed
 
-lemma [simp]: "map_option f \<circ> map_option g \<circ> h = map_option (f \<circ> g) \<circ> h"
-  by (rule, auto, metis option.map_comp)
-
-lemma [simp]: "map_option f \<circ> (map_option g \<circ> h) = map_option (f \<circ> g) \<circ> h"
-  by (rule, auto, metis option.map_comp)
-
-lemma [simp]: "length as = length bs \<Longrightarrow> 
+lemma list_all_zip [simp]: "length as = length bs \<Longrightarrow> 
   list_all (\<lambda>(a, b). P a \<and> Q b) (zip as bs) = (list_all P as \<and> list_all Q bs)"
 proof (induction as arbitrary: bs)
   case (Cons a as)
   thus ?case by (induction bs) auto
 qed simp_all
 
-abbreviation nmem :: "nat \<Rightarrow> 'a" where
-  "nmem x \<equiv> undefined"
-
-lemma [simp]: "(a # as @ bs) ! length as = (a # as) ! length as"
-  by (induction as arbitrary: a) simp_all
-
-lemma [simp]: "0 < x \<Longrightarrow> x \<le> length as \<Longrightarrow> (as @ bs) ! (length as - x) = as ! (length as - x)"
-proof (induction as arbitrary: x bs rule: rev_induct)
-  case (snoc a as)
-  thus ?case 
-  proof (induction x)
-    case (Suc x)
-    thus ?case by (induction x) simp_all
-  qed simp_all
-qed simp_all
-
-lemma [simp]: "length (concat (replicate x as)) = length as * x"
+lemma length_concat_replicate [simp]: "length (concat (replicate x as)) = length as * x"
   by (induction x) simp_all
 
-lemma [simp]: "map f (concat (replicate x as)) = concat (replicate x (map f as))"
+lemma map_concat_replicate [simp]: "map f (concat (replicate x as)) = 
+    concat (replicate x (map f as))"
   by (induction x) simp_all
 
-lemma [simp]: "map prod.swap (zip as bs) = zip bs as"
-proof (induction as arbitrary: bs)
-  case (Cons a as)
-  thus ?case by (induction bs) simp_all
-qed simp_all
-
-lemma [simp]: "x < y \<Longrightarrow> 1 < k \<Longrightarrow> Suc (k * x) < k * y"
+lemma suc_mult_lt_lemma [simp]: "x < y \<Longrightarrow> 1 < k \<Longrightarrow> Suc (k * x) < k * y"
   by (metis One_nat_def Suc_lessE Suc_lessI Suc_mult_less_cancel1 Suc_times_mod_eq 
             mod_mult_self1_is_0 nat.simps(3))
+
+lemma x_mod_3_induct [case_names 0 1 2]: "((x::nat) mod 3 = 0 \<Longrightarrow> P x) \<Longrightarrow> (x mod 3 = 1 \<Longrightarrow> P x) \<Longrightarrow> 
+    (x mod 3 = 2 \<Longrightarrow> P x) \<Longrightarrow> P x"
+  by linarith
 
 end
